Issue with new while

src/phl/ecPhlSp.ml
@@ -39,6 +39,48 @@ open EcLowPhlGoal
  *   2) $MISSING...
  *)
 
+
+(* -------------------------------------------------------------------- *)
+let pp_encapsulate fmt pp_fun msg =
+  let _ = Format.pp_force_newline fmt (Format.pp_print_string fmt "--------------------------------------------------------------------") in
+  let _ = Format.pp_force_newline fmt (Format.pp_print_string fmt msg) in
+  let _ = Format.pp_force_newline fmt (Format.pp_print_string fmt "--------------------------------------------------------------------") in
+  let _ = pp_fun fmt in
+  let _ = Format.pp_force_newline fmt (Format.pp_print_string fmt "--------------------------------------------------------------------") in
+  Format.pp_force_newline fmt ()
+
+let pp_stmt_completed env stmt msg =
+  let lineno = true in
+  let ppenv = EcPrinting.PPEnv.ofenv env in
+  let fmt = Format.std_formatter in
+  (*Why do I have to give a specific name to the optional argument?*)
+  pp_encapsulate fmt (fun fmt -> EcPrinting.pp_stmt ~lineno ppenv fmt stmt) msg
+
+let pp_hs_completed env hs msg =
+  let ppenv = EcPrinting.PPEnv.ofenv env in
+  let fmt = Format.std_formatter in
+  pp_encapsulate fmt (fun fmt -> EcPrinting.pp_hoareS ppenv fmt hs) msg
+
+let pp_bhs_completed env bhs msg =
+  let ppenv = EcPrinting.PPEnv.ofenv env in
+  let fmt = Format.std_formatter in
+  pp_encapsulate fmt (fun fmt -> EcPrinting.pp_bdhoareS ppenv fmt bhs) msg
+
+let pp_pvs env pvs msg =
+  let ppenv = EcPrinting.PPEnv.ofenv env in
+  let fmt = Format.std_formatter in
+  pp_encapsulate fmt (fun fmt -> List.iter (fun pv -> Format.pp_force_newline fmt (EcPrinting.pp_pv ppenv fmt pv)) pvs) msg
+
+let pp_pvt_of_instr env instr msg =
+  let modi = EcPV.i_write env instr in
+  let fmt = Format.std_formatter in
+  pp_encapsulate fmt (fun fmt -> Format.pp_force_newline fmt (EcPV.PV.pp env fmt modi)) msg
+
+let pp_pvt_of_stmt env stmt msg =
+  let modi = EcPV.s_write env stmt in
+  let fmt = Format.std_formatter in
+  pp_encapsulate fmt (fun fmt -> Format.pp_force_newline fmt (EcPV.PV.pp env fmt modi)) msg
+
 (* -------------------------------------------------------------------- *)
 module LowInternal = struct
   (* ------------------------------------------------------------------ *)
@@ -182,28 +224,30 @@ module LowInternal = struct
     EcCoreFol.f_fold aux [] pre
 
   let sp_instr_free env pre instr =
+    (*pp_pvt_of_instr env instr "Printing prog_vars written on in program seen by sp";*)
     let modi = EcPV.i_write env instr in
-    let aux pv = if not (EcPV.PV.mem_pv env pv modi) then raise No_sp in
+    let aux pv = if (EcPV.PV.mem_pv env pv modi) then raise No_sp in
     List.iter aux (pvs_of_form pre)
 
   (* ------------------------------------------------------------------ *)
-  let rec sp_stmt m env (bds, assoc, pre) stmt =
+  let rec sp_stmt p m env (bds, assoc, pre) stmt =
     match stmt with
     | [] ->
         ([], (bds, assoc, pre))
 
     | i :: is ->
         try
-          let _ = sp_instr_free env pre i in
-          sp_stmt m env (bds,assoc,pre) is
+          if p then raise No_sp;
+          sp_instr_free env pre i;
+          sp_stmt p m env (bds,assoc,pre) is
         with No_sp ->
           try
-            let (bds, assoc, pre) = sp_instr m env (bds, assoc, pre) i in
-            sp_stmt m env (bds,assoc,pre) is
+            let (bds, assoc, pre) = sp_instr p m env (bds, assoc, pre) i in
+            sp_stmt p m env (bds,assoc,pre) is
           with No_sp ->
             (stmt, (bds, assoc, pre))
 
-  and sp_instr m env (bds,assoc,pre) instr = match instr.i_node with
+  and sp_instr p m env (bds,assoc,pre) instr = match instr.i_node with
     | Sasgn (lv, e) ->
         sp_asgn m env lv e (bds, assoc, pre)
 
@@ -211,8 +255,8 @@ module LowInternal = struct
         let e_form = EcFol.form_of_expr m e in
         let pre_t  = build_sp m bds assoc (f_and_simpl e_form pre) in
         let pre_f  = build_sp m bds assoc (f_and_simpl (f_not e_form) pre) in
-        let stmt_t, (bds_t, assoc_t, pre_t) = sp_stmt m env (bds, assoc, pre_t) s1.s_node in
-        let stmt_f, (bds_f, assoc_f, pre_f) = sp_stmt m env (bds, assoc, pre_f) s2.s_node in
+        let stmt_t, (bds_t, assoc_t, pre_t) = sp_stmt p m env (bds, assoc, pre_t) s1.s_node in
+        let stmt_f, (bds_f, assoc_f, pre_f) = sp_stmt p m env (bds, assoc, pre_f) s2.s_node in
         if not (List.is_empty stmt_t && List.is_empty stmt_f) then raise No_sp;
         let sp_t = build_sp m bds_t assoc_t pre_t in
         let sp_f = build_sp m bds_f assoc_f pre_f in
@@ -220,8 +264,8 @@ module LowInternal = struct
 
     | _ -> raise No_sp
 
-  let sp_stmt m env stmt f =
-    let stmt, (bds, assoc, pre) = sp_stmt m env ([], [], f) stmt in
+  let sp_stmt p m env stmt f =
+    let stmt, (bds, assoc, pre) = sp_stmt p m env ([], [], f) stmt in
     let pre = build_sp m bds assoc pre in
     stmt, pre
 end
@@ -259,14 +303,22 @@ let t_sp_side pos tc =
 
   match concl.f_node, pos with
   | FhoareS hs, (None | Some (Single _)) ->
+      (*
+      pp_pvs env (LI.pvs_of_form hs.hs_pr) "Printing prog_vars in precondition";
+      pp_pvt_of_stmt env hs.hs_s "Printing prog_vars written on in program";
+      *)
       let pos = pos |> omap as_single in
       let stmt1, stmt2 = o_split ~rev:true pos hs.hs_s in
-      let stmt1, hs_pr = LI.sp_stmt (EcMemory.memory hs.hs_m) env stmt1 hs.hs_pr in
+      let stmt1, hs_pr = LI.sp_stmt false (EcMemory.memory hs.hs_m) env stmt1 hs.hs_pr in
       check_sp_progress pos stmt1;
       let subgoal = f_hoareS_r { hs with hs_s = stmt (stmt1@stmt2); hs_pr } in
       FApi.xmutate1 tc `Sp [subgoal]
 
   | FbdHoareS bhs, (None | Some (Single _)) ->
+      (*
+      pp_pvs env (LI.pvs_of_form bhs.bhs_pr) "Printing prog_vars in precondition";
+      pp_pvt_of_stmt env bhs.bhs_s "Printing prog_vars written on in program";
+      *)
       let pos = pos |> omap as_single in
       let stmt1, stmt2 = o_split ~rev:true pos bhs.bhs_s in
       begin
@@ -275,7 +327,7 @@ let t_sp_side pos tc =
         if not (EcPV.PV.indep env write_set read_set) then
           tc_error !!tc "the bound should not be modified by the statement targeted by [sp]"
       end;
-      let stmt1, bhs_pr = LI.sp_stmt (EcMemory.memory bhs.bhs_m) env stmt1 bhs.bhs_pr in
+      let stmt1, bhs_pr = LI.sp_stmt true (EcMemory.memory bhs.bhs_m) env stmt1 bhs.bhs_pr in
       check_sp_progress pos stmt1;
       let subgoal = f_bdHoareS_r {bhs with bhs_s = stmt (stmt1@stmt2); bhs_pr; } in
       FApi.xmutate1 tc `Sp [subgoal]
@@ -289,8 +341,8 @@ let t_sp_side pos tc =
       let stmtR1, stmtR2 = o_split ~rev:true posR es.es_sr in
 
       let         es_pr = es.es_pr in
-      let stmtL1, es_pr = LI.sp_stmt (EcMemory.memory es.es_ml) env stmtL1 es_pr in
-      let stmtR1, es_pr = LI.sp_stmt (EcMemory.memory es.es_mr) env stmtR1 es_pr in
+      let stmtL1, es_pr = LI.sp_stmt true (EcMemory.memory es.es_ml) env stmtL1 es_pr in
+      let stmtR1, es_pr = LI.sp_stmt true (EcMemory.memory es.es_mr) env stmtR1 es_pr in
 
       check_sp_progress ~side:`Left  pos stmtL1;
       check_sp_progress ~side:`Right pos stmtR1;
