examples/sp_free.ec
@@ -2,6 +2,10 @@ require import AllCore Int StdOrder.
 import IntOrder.
 
 module MAIN = {
+  proc incr (n : int) : int = {
+    n <- n + 1;
+    return n;
+  }
   proc id_while (n : int) : int = {
     var i;
     i <- 0;
@@ -17,35 +21,14 @@ module MAIN = {
   }
 }.
 
+lemma incr_free m :
+  hoare [MAIN.incr : n = m ==> res = m + 1].
+proof. by proc; sp; skip. qed.
+
 lemma id_while_free m :
   hoare [MAIN.id_while : m = 0 ==> m = 0].
 proof. by proc; sp; skip. qed.
 
 lemma id_call_free m :
   hoare [MAIN.id_call : m = 0 ==> m = 0].
-proof. by proc; sp; skip. qed.
-
-module FALSE = {
-  proc incr (n : int) : unit = {
-    n <- n + 1;
-    return ();
-  }
-  proc incr_call (n : int) : int = {
-    incr(n);
-    return n;
-  }
-  proc infinite () : unit = {
-    while(true) {}
-    return ();
-  }
-}.
-
-(*Interesting, does s_write unfold function calls?*)
-lemma incr_call_free m :
-  hoare [FALSE.incr_call : n = m ==> res = m].
-proof. proc. sp. abort.
-
-(*This is really bad.*)
-lemma islossless_infinite_free :
-  islossless FALSE.infinite.
 proof. by proc; sp; skip. qed.
